Added Init to CIVL solution and lots of comments

civl.bpl
@@ -1,13 +1,86 @@
+// This is a specification of a simple concurrent algorithm from the paper
+// "Teaching Concurrency" by Leslie Lamport. In there are N processes and
+// two arrays of length N, x and y. Each process i executes the following
+// sequence of statements:
+//
+//     x[i] := 1;
+//     y[i] := x[(i-1) mod N];
+//
+// The reads and writes of each x[j] are assumed to be atomic. This
+// algorithm has the property that once all processes have finished, at
+// least one y[j] == 1.
+//
+// The algorithm is specified with an Init which specifies the initial
+// state of the system and a Proc method which specifies the above instructions
+// and has some assertions after each yield to prove correctness.
+//
+// Unlike in all other tools I've tried (TLA+, Dafny, Mypyvy), it wasn't
+// necessary to record the control state of each process in a variable.
+// Instead, I only record a boolean for each process, indicating whether
+// that process has completed. This surprised me because the inductive
+// invariant requires recording that if a process has completed the x
+// update, its value of x is equal to 1. I weakened this part of the
+// inductive invariant to just say that if a process has finished, then
+// its value of x is equal to 1. I think CIVL is able to handle this weaker
+// inductive invariant because I added an assertion that x[i] == 1 after
+// the yield following the x update step. This seems to be, in some sense,
+// a local way of recording the information that is missing from the
+// inductive invariant. So the inductive invariant is spread between the
+// predicate I've named ind_inv and this local assertion. As far as I can tell,
+// this is the only fundamentally different proof of this algorithm in the
+// different tools that I've tried.
+//
+// One shouldn't take the above discussion too seriously. I don't really
+// understand CIVL, so I'm not sure if I've really specified/verified what
+// I think I have.
+//
+// As with the Dafny solution, there is no scheduler method that actually
+// calls Init and Proc, so there's no complete verification result, only
+// an implicit one. I suspect that it's possible to write such a scheduler,
+// but I don't know enough about CIVL to do so.
+
+// Number of processes in the algorithm. There needs to be at least one.
 const N : int;
 axiom N >= 1;
 
 var {:layer 0} x : [int]int;
 var {:layer 0} y : [int]int;
-// ghost variable recording completion of
-// a process. I don't see how to do this without
-// such a variable.
-var {:layer 0} done : [int]bool; 
+// Records whether or not a process has finished.
+var {:layer 0} done : [int]bool;
 
+// Initial state of the system
+procedure {:layer 0} Init()
+ensures ind_inv(done, y, x);
+modifies done, y, x;
+{
+	// Only the initial value of pc matters.
+  done := (lambda i: int :: false);
+	// Convince boogie that at least one process is not done.
+  assert !done[0];
+}
+
+// The specification of a process, along with post-yield
+// assertions necessary to conclude ind_inv.
+procedure {:yields}	{:layer 0} Proc(i: int)
+requires {:layer 0} ind_inv(done, y, x);
+ensures {:layer 0} ind_inv(done, y, x);	
+{
+  call update_x(i);
+	yield;
+	assert {:layer 0} x[i] == 1;
+	assert {:layer 0} x_inv(done, x);
+	assert {:layer 0} safety(done, y);
+
+	call update_y(i);
+	call mark_done(i);
+	yield;
+	assert {:layer 0} x_inv(done, x);
+	assert {:layer 0} safety(done, y);	
+}
+
+// CIVL doesn't seem to allow updates of global variables
+// within yielding procedures, so I have to put these
+// updates in non-yielding procedures.
 procedure {:layer 0} update_x(i: int)
 modifies x;
 ensures x == old(x)[i:=1];
@@ -29,108 +102,33 @@ ensures done == old(done)[i:=true];
   done := done[i:=true];
 }	
 
+// Whether or not an int i indicates an actual process
 function in_range(i: int): bool
 {
 	0 <= i && i < N
 }	
 
-function inv(done: [int]bool, y: [int]int): bool
+// The core correctness property of the system. If all the processes
+// have finished, there's at least one element of y equal to 1.
+function safety(done: [int]bool, y: [int]int): bool
 {
 	(forall i : int :: in_range(i) ==>  done[i]) ==>
 	(exists i : int :: (in_range(i) && y[i] == 1))
 }
 
+// Records that all completed processes have their x equal to 1.
+// This is weaker than than to corresponding inductive invariant
+// conjunct in other tools for the same algorithm.
 function x_inv(done: [int]bool, x: [int]int): bool
 {
 	(forall i : int :: (in_range(i) && done[i]) ==>  x[i] == 1)
 }
 
+// Inductive invariant. Given the discussion at the top of this file,
+// this should probably be considered part of the global inductive
+// invariant. I think the assert x[i] == 1 in Proc is also, in some sense,
+// part of the global inductive invariant.
 function ind_inv(done: [int]bool, y: [int]int, x: [int]int): bool
 {
-  inv(done, y) && x_inv(done, x)
+  safety(done, y) && x_inv(done, x)
 }
-
-procedure {:yields}	{:layer 0} run(i: int)
-requires {:layer 0} ind_inv(done, y, x);
-ensures {:layer 0} ind_inv(done, y, x);	
-{
-  call update_x(i);
-	yield;
-	assert {:layer 0} x[i] == 1;
-	assert {:layer 0} x_inv(done, x);
-	assert {:layer 0} inv(done, y);
-
-	call update_y(i);
-	call mark_done(i);
-	assert {:layer 0} x_inv(done, x);
-	assert {:layer 0} inv(done, y);
-}
-
-// Once I just added the done variable and encoded the inductive invariant
-// and asserted it everywhere, everything just
-// worked. Main downside is I can't figure out
-// how to write a "main" procedure to get an
-// end to end result. This is probably my own
-// ignorance and a lack of documentation.
-//
-// The stated inductive invariant is split in a sense, relative
-// to TLA+ - there's an assert (x[i] == 1) which is covered
-// by pc[i] == "s2" => x[i] = 1 in the TLA+ inductive invariant.
-//
-// I generally wasn't sure what to do when something didn't get
-// verified. In TLA+, I can just decompose the proof further.
-// The analogous thing here seems to be adding assertions, but
-// that's a flat approach, doesn't seem to allow decomposition.
-// It's an unfair comparison because I have decent experience
-// writing TLA+ proofs and almost no experience with CIVL. And,
-// once I got the hang of assertion-based proof debugging, it
-// worked out reasonably well for this simple example.
-//
-// Unlike TLAPS, there are counter example traces, but they mean
-// nothing to me, so it is as good as no counter example.
-//
-// When I first started this proof, I tried to express only local
-// assertions/contracts, but it wasn't clear how to do so. This
-// problem seems to inherently requires some form of global
-// reasoning.
-// Example:
-// - try a ghost variable to record value of x_left before the
-//   y step (I wasn't sure what to do with this variable).
-// - try ensure that either y[i] == 1 or left proc not done
-//   (a form of global reasoning).
-//
-// Assertions within the program text was maybe a bit faster
-// than in TLAPS, but it's hard to say how well that would scale
-// to more complicated examples.
-//
-// One problem is that I don't really understand what get checked
-// at each yield point.
-//
-// Annoying that I have to factor out update_x and update_y.
-
-procedure {:yields}	{:layer 0} run_all(i: int)
-requires {:layer 0} 0 <= i && i <= N;
-requires {:layer 0} ind_inv(done, y, x);
-ensures {:layer 0} ind_inv(done, y, x);
-{
-	if (i < N) {
-		 par run(i) | run_all(i + 1);
-	}
-	yield;
-}	
-
-// Assertion based proof debugging kind of nice.
-// Hard to say how it would work when more levels
-// might be required.
-procedure {:yields}	{:layer 0} main()
-requires {:layer 0} (forall i : int :: in_range(i) ==>  !done[i]);
-ensures {:layer 0} ind_inv(done, y, x);
-{
-	// Need this assertion, probably to prove
-	// that there exists an i in_range.
-  assert {:layer 0} in_range(0);
-	call run_all(0);
-//  par run(0);// | run(1);
-	yield;
-	assert {:layer 0}	ind_inv(done, y, x);
-}	
